liveness analysis, use list notation, fix inst_args

core/LivenessAnalysis.v
@@ -1,6 +1,8 @@
 From Ssara.Core Require Import Syntax.
 From Ssara.Core Require Import Vm.
 From Stdlib Require Import Lists.List.
+From Stdlib Require Import ZArith.
+Import ListNotations.
 
 (*
   https://en.wikipedia.org/wiki/Live-variable_analysis
@@ -11,19 +13,23 @@ Inductive metainst : Type :=
 .
 
 CoInductive metablock : Type :=
-  | Metablock (ms : list metainst) (succ : list metablock)
+  | Metablock (phi_args: list reg) (ms : list metainst) (succ : list metablock)
 .
 
 Definition contains (x : reg) (xs : list reg) : bool :=
   existsb (fun n => Nat.eqb x n) xs
 .
 
-Fixpoint reg_union (regs : list reg) (regs' : list reg) : list reg :=
+Fixpoint regs_union (regs : list reg) (regs' : list reg) : list reg :=
   match regs' with
   | nil => regs
   | x :: xs =>
-    if contains x regs then reg_union regs xs else x :: reg_union regs xs
+    if contains x regs then regs_union regs xs else x :: regs_union regs xs
   end
+.
+
+Notation "x 'U' y" :=
+  (regs_union x y) (at level 50)
 .
 
 Fixpoint remove (r : reg) (regs : list reg) : list reg :=
@@ -34,10 +40,10 @@ Fixpoint remove (r : reg) (regs : list reg) : list reg :=
   end
 .
 
-Fixpoint reg_minus (regs : list reg) (regs' : list reg) : list reg :=
+Fixpoint regs_minus (regs : list reg) (regs' : list reg) : list reg :=
   match regs' with
   | nil => regs
-  | x :: xs => reg_minus (remove x regs) xs
+  | x :: xs => regs_minus (remove x regs) xs
   end
 .
 
@@ -52,14 +58,55 @@ Definition option_to_list {A : Type} (x : option A) : list A :=
   Liveness analysis of a phi instruction
   - use[i]      := empty
   - def[i]      := reg[i]
-  - live_out[i] := U in[j] with j ∈ succ[i]
-  - live_in[i]  := use[i] U (out[i] - def[i])
+  - live_out[i] := U with j ∈ succ[i] of (live_in[j] U args[j])
+  - live_in[i]  := use[i] U (live_out[i] - def[i])
+
+  Where final_live_out is the live_out of the last phi instruction, which is in
+  function of the successor succ[final] which is either an inst or a jinst
+*)
+
+Fixpoint analyze_phis
+  (ps : list phi)
+  (final_live_out : list reg)
+  : (list metainst) * (list reg) :=
+  match ps with
+  | nil => (nil, final_live_out)
+  | x :: xs =>
+    let def := option_to_list (phi_reg x) in
+    let (ps', live_out) := analyze_phis xs final_live_out in
+    let live_in := (regs_minus live_out def) in (
+      (Metainst nil def live_out live_in) :: ps',
+      live_in U (phi_args x)
+    )
+  end
+.
+
+Module Example1.
+  Definition ps: list phi := [
+      r(0) <- phi [3; 4; 5];
+      r(1) <- phi [6; 7; 8];
+      r(2) <- phi [9; 10; 11]
+    ]
+  .
+
+  Compute analyze_phis ps nil.
+End Example1.
+
+(*
+  Liveness analysis of a generic instruction
+  - use[i]      := args[i]
+  - def[i]      := reg[i]
+  - live_out[i] := U live_in[j] with j ∈ succ[i]
+  - live_in[i]  := use[i] U (live_out[i] - def[i])
 *)
 
 (*
   This generic function is used to get the metadata of a section of
   instructions, it takes in the generic arguments, the list of instructions and
-  the final live_out set which is live_out[final] := U in[j] with j ∈ succ[i]
+  the final live_out set which is live_out[final] := U in[j] with j ∈ succ[i].
+  NOTE: the difference between analyze_As and analyze_phis is that, even though
+  in both cases the arguments of the instruction are passed to the predecessor
+  the phi instruction does not define use as the set of its arguments.
 *)
 
 Fixpoint analyze_As
@@ -75,20 +122,27 @@ Fixpoint analyze_As
     let use := get_args x in
     let def := get_reg x in
     let (is', live_out) := analyze_As get_reg get_args xs final_live_out in
-    let live_in := reg_union use (reg_minus final_live_out def) in (
+    let live_in := use U (regs_minus final_live_out def) in (
       (Metainst use def final_live_out live_in) :: is',
       live_in
     )
   end
 .
 
-Definition analyze_phis (ps : list phi) (final_live_out : list reg) : list metainst * list reg :=
-  analyze_As (fun x => option_to_list (phi_reg x)) (fun _ => nil) ps final_live_out
-.
-
 Definition analyze_insts (is : list inst) (final_live_out : list reg) : list metainst * list reg :=
   analyze_As (fun x => option_to_list (inst_reg x)) inst_args is final_live_out
 .
+
+Module Example2.
+  Definition is : list inst := [
+      r(0) <- r(1) + (Imm 1)
+    ]
+  .
+
+  Compute inst_args (r(0) <- r(1) + (Imm 1)).
+
+  Compute analyze_insts is nil.
+End Example2.
 
 Definition analyze_jinst (j : jinst) (final_live_out : list reg) : list metainst * list reg :=
   analyze_As (fun _ => nil) (fun x => option_to_list (jinst_args x)) (j :: nil) final_live_out
@@ -97,19 +151,32 @@ Definition analyze_jinst (j : jinst) (final_live_out : list reg) : list metainst
 Definition analyze_block (b : block) (final_live_out : list reg) : list metainst * list reg :=
   match b with
   | Block ps is j =>
-    let (m_1, final_live_out_1) := analyze_jinst j final_live_out in
-    let (m_2, final_live_out_2) := analyze_insts is final_live_out_1 in
-    let (m_3, final_live_out_3) := (analyze_phis ps final_live_out_2) in
-    (m_1 ++ m_2 ++ m_3, final_live_out_3)
+    let (m_3, final_live_out_3) := analyze_jinst j final_live_out in
+    let (m_2, final_live_out_2) := analyze_insts is final_live_out_3 in
+    let (m_1, final_live_out_1) := (analyze_phis ps final_live_out_2) in
+    (m_1 ++ m_2 ++ m_3, final_live_out_1)
   end
 .
 
-(* Definition analyze_program (p : program) : list metainst * list reg :=
+Module Example3.
+  Definition example_block : block := Block [
+      r(0) <- phi [1; 2; 3]
+    ] [
+      r(4) <- r(0) + (Imm 1)
+    ] (
+      Halt
+    )
+  .
+
+  Compute analyze_block example_block nil.
+End Example3.
+
+(*
+Definition analyze_program (p : program) : list metainst * list reg :=
   match p with
   | x :: nil => analyze_block
-  |  *)
+  |
 
-(* 
 Fixpoint analyze_block : (b : block) (live_in : list reg) : metablock :=
   match b with
   | nil =>  *)
