test/Test.v
@@ -4,35 +4,36 @@ From Stdlib Require Import Lists.List.
 From Stdlib Require Import ZArith.
 From Stdlib Require Import Bool.
 From QuickChick Require Import QuickChick.
+Import ListNotations.
 
 (* Example 1 *)
 
 Module Example1.
   Definition example_block : block :=
-    Block (
-      nil
-    ) (
-      (r(2) <- (Imm 34)) ::
-      (r(3) <- r(2) * (Imm 2)) ::
-      (r(4) <- r(3) + (Imm 1)) ::
-      (store (Ptr 5) r(4)) ::
-      (r(5) <- load (Ptr 5)) ::
-      (r(6) <- r(4) < (Imm 420)) ::
-      nil
-    ) (
+    Block [
+    ] [
+      r(2) <- (Imm 34);
+      r(3) <- r(2) * (Imm 2);
+      r(4) <- r(3) + (Imm 1);
+      store (Ptr 5) r(4);
+      r(5) <- load (Ptr 5);
+      r(6) <- r(4) < (Imm 420)
+    ] (
       Halt
     )
   .
 
   Example run_example :
     run_aux (Vm nil nil) example_block 1 =
-      Vm ((2, 34%Z) :: (3, 68%Z) :: (4, 69%Z) :: (5, 69%Z) :: (6, 1%Z) :: nil)
-      (0%Z :: 0%Z :: 0%Z :: 0%Z :: 0%Z :: 69%Z :: nil)
+      Vm [(2, 34%Z); (3, 68%Z); (4, 69%Z); (5, 69%Z); (6, 1%Z)]
+      [0%Z; 0%Z; 0%Z; 0%Z; 0%Z; 69%Z]
   .
   Proof.
     reflexivity.
   Qed.
 End Example1.
+
+(* Example 2 *)
 
 Module Exmaple2.
   CoFixpoint example_block_1 :=
@@ -51,50 +52,44 @@ End Exmaple2.
 
 Module Example3.
   Definition example_block_1 : block :=
-    Block (
-      (r(2) <- phi (0 :: 1 :: nil)) ::
-      nil
-    ) (
-      (store (Ptr 0) r(2)) ::
-      nil
-    ) (
+    Block [
+      r(2) <- phi [0; 1]
+    ] [
+      store (Ptr 0) r(2)
+    ] (
       Halt
     )
   .
 
   Definition example_block_2 : block :=
-    Block (
-      nil
-    ) (
-      (r(0) <- (Imm 34)) ::
-      nil
-    ) (
+    Block [
+    ] [
+      r(0) <- (Imm 34)
+    ] (
       Jmp example_block_1
     )
   .
 
   Definition example_block_3 : block :=
-    Block (
-      nil
-    ) (
-      (r(1) <- (Imm 35)) ::
-      nil
-    ) (
+    Block [
+    ] [
+      r(1) <- (Imm 35)
+    ] (
       Jmp example_block_1
     )
   .
 
   Example run_example_1 :
-    Vm.run (Vm nil nil) (example_block_3 :: example_block_2 :: example_block_1 :: nil) 10
-    = Vm ((1, 35%Z) :: (2, 35%Z) :: nil) (35%Z :: nil)
+    Vm.run (Vm nil nil) [example_block_3; example_block_2; example_block_1] 10
+    = Vm [(1, 35%Z); (2, 35%Z)] [35%Z]
   .
   Proof.
     reflexivity.
   Qed.
 
   Example run_example_2 :
-    Vm.run (Vm nil nil) (example_block_2 :: example_block_3 :: example_block_1 :: nil) 10
-    = Vm ((0, 34%Z) :: (2, 34%Z) :: nil) (34%Z :: nil)
+    Vm.run (Vm nil nil) [example_block_2; example_block_3; example_block_1] 10
+    = Vm [(0, 34%Z); (2, 34%Z)] [34%Z]
   .
   Proof.
     reflexivity.
@@ -123,7 +118,7 @@ QuickChick set_reg_P.
 *)
 Definition store_P (i : nat) (c : cell) : bool :=
   let m := Vm nil nil in
-  let p := (Block nil ((r(0) <- (Imm c)) :: (store (Ptr i) r(0)) :: nil) Halt) :: nil in
+  let p := [(Block nil [r(0) <- (Imm c); store (Ptr i) r(0)] Halt)] in
   let (_, cells) := Vm.run m p 10 in
   match nth_error cells i with
   | Some c' => Z.eqb c c'
